#+HTML_HEAD: <link rel="stylesheet" href="http://xieyuheng.github.io/asset/css/page.css" type="text/css" media="screen" />
#+title: 項格

* lattice

  - a cover b
    b under a

* example of lattice

  - natural number
    with gcd as meet
    number better viewed as been fully factorized to prime

  - convex figure in space
    [topological space]

  - linear term lattice

  - term lattice

* ><

  - 在引入具體的 項格 時
    需要用 棧傳遞函數來實現其中的基本關係與基本運算
    還需要 env passing

  - 注意對等詞的處理

  - 當考慮分解好的自然數時
    數就類似 term 了
    而 求 gcd 的過程 就類似 unification

* [EWD1240a] a little bit of lattice theory

  - *type-constructor*
    (<lattice> = <lattice>)
    (<lattice> under <lattice>)
  - *axiom*
    reflexive of under
    (x : <lattice> -> (x under x))
  - the following proposition is equal to reflexive
    (x y : <lattice> (x = y) -> (x under y) (y under x))
    one-point-rule
    (x x : <lattice> (x = x) -> (x under x) (x under x))
    drop
    (x : <lattice> -> (x under x))
  - *axiom*
    antisymmetric of under
    (x y : <lattice> (x under y) (y under x) -> (x = y))
  - by reflexive of under
    we can proof indirect under
    1. ((x y z : <lattice> (z under x) -> (z under y)) -> (x under y))
    2. ((x y z : <lattice> (y under z) -> (x under z)) -> (x under y))
    proof 1
    (x y z : <lattice> (z under x) -> (z under y))
    instantiate
    (x y x : <lattice> (x under x) -> (x under y))
    reflexive of under
    (x y x : <lattice> true -> (x under y))
    drop
    (x y : <lattice> -> (x under y))
    end proof
  - by antisymmetric of under
    we can proof indirect equal
    1. ((x y z : <lattice> (z under x) <-> (z under y)) -> (x = y))
    2. ((x y z : <lattice> (y under z) <-> (x under z)) -> (x = y))
    proof 1
    (x y z : <lattice> (z under x) <-> (z under y))
    instantiate 2 times
    (x y : <lattice>  ((x under x) <-> (x under y))  ((y under x) <-> (y under y)))
    reflexive of under
    (x y : <lattice>  (true <-> (x under y))  ((y under x) <-> true))
    drop
    (x y : <lattice>  (x under y)  (y under x))
    antisymmetric of under
    (x y : <lattice>  (x = y))
    end proof
  - *axiom*
    the existence of w
    use under to define join [up] [lowest upper bound] [superemum]
    (x y : <lattice> -> w : <lattice> (z : <lattice> -> ((w under z) <-> (x under z) (y under z))))
    define
    (x y : <lattice> -> (x join y))
    or
    (x y : <lattice> -> w : (x join y))
    a new type constructor is defined
    need to proof w is unique
    to view this type constructor as function
  - join
    1. idempotent
       (x join x) = x
    2. symmetry
       (x join y) = (y join x)
    3. associative
       ((x join y) join z) = (x join (y join z))
    proof associative
    ><><><
    end proof
  - wish to proof
    (x y : <lattice> ((x join y) = y) <-> (x under y))
    and use it to proof the transitive of under
    (x y z : <lattice> (x under y) (y under z) -> (x under z))
    thus under is partial-order
    1. reflexive
    2. antisymmetric
    3. transitive

* ><

  #+begin_src scheme
  (lattice

   cover (lattice lattice -> type)
   reflexive ((:x : lattice) -> :x :x cover)
   antisymmetry
   ((:x :y : lattice)
    :x :y cover :y :x cover
    ------------------->
    :x :y equal)
   ;; maybe it is the very definition of equal
   ;; that maintaining this proposition
   indirect-cover
   (((:z : lattice) :z :x cover -> :z :y cover)
    ---------------->
    :x :y cover)
   indirect-cover'
   (((:z : lattice) :y :z cover -> :x :z cover)
    ---------------->
    :x :y cover)

   meet (lattice lattice -> lattice)
   join (lattice lattice -> lattice)
   idempotent
   ((:x : lattice) -> :x :x meet :x equal)
   symmetry
   ((:x :y : lattice) -> :x :y meet :y :x meet equal)
   associative
   (-> :x :y meet :z meet
       :x :y :z meet meet
       equal))

  ((:x : lattice) -> :x :x cover)

  ;; use the follow theorem reflexive2 to proof reflexive

  (defn reflexive2
      ((:x :y : lattice) :x :y equal -> :y :x cover :x :y cover)
    ><><><)

  ((:x :y : lattice)
   :x :y cover :y :x cover
   <------------------->
   :x :y equal)

  (defn same-equal-same
      (:x :x -> :x :x equal)
    ><><><)

  (defn reflexive ((:x : lattice) -> :x :x cover)
    (:d -> dup dup2 same-equal-same reflexive2 drop))
  #+end_src
